Restructure, prove typing-configs-disjoint theorem

TypingContexts.v
@@ -4,8 +4,7 @@ From Coq Require Import MSets.
 Import ListNotations.
 Require Import List.
 Require Import lang_spec.
-
-Module VarSet := Make(Nat_as_OT).
+Require Import VarSet.
 
 Inductive Judgement : Type :=
 | judge (v : var) (t : type)
@@ -13,18 +12,12 @@ Inductive Judgement : Type :=
 
 Definition ty_ctx := (list Judgement).
 
-Definition disj_vars (s1 s2 : VarSet.t) := VarSet.Empty (VarSet.inter s1 s2).
-
 (* Functions to convert between the different types listed above *)
-
-Fixpoint var_to_varset (v : var) : VarSet.t :=
-  VarSet.singleton v.
-Coercion var_to_varset : var >-> VarSet.t.
 
 Fixpoint bound_variables (g : ty_ctx) : VarSet.t :=
   match g with
   | nil => VarSet.empty
-  | cons (judge v _) g' =>VarSet.union (VarSet.singleton v) (bound_variables g')
+  | cons (judge v _) g' => VarSet.union (VarSet.singleton v) (bound_variables g')
   end.
 Coercion bound_variables : ty_ctx >-> VarSet.t.
 
@@ -36,7 +29,6 @@ Definition ctx_union (g1 g2 : ty_ctx) (disjoint_proof : disj_vars g1 g2) : ty_ct
 Fixpoint coerce_judgement_to_ty_ctx (j : Judgement) : ty_ctx :=
   cons j nil.
 Coercion coerce_judgement_to_ty_ctx : Judgement >-> ty_ctx.
-
 
 Fixpoint eq (n m : nat) : bool :=
   match n, m with
@@ -55,40 +47,21 @@ Fixpoint restrict_ty_ctx (g : ty_ctx) (x : var) : ty_ctx :=
 
 Notation "g -- x" := (restrict_ty_ctx g x) (at level 71, left associativity).
 
-Theorem axiom_restriction_commutative :
+Theorem restriction_commutative :
   forall g : ty_ctx,
   forall v1 v2 : var,
   (g -- v1 -- v2) = (g -- v2 -- v1).
 Proof. Admitted.
 
+Theorem restriction_makes_subset :
+  forall g : ty_ctx,
+  forall v : var,
+    VarSet.Subset (g -- v) g.
+Proof. Admitted.
+
 (* Set-Theory Theorems: warning a lot of admits are gonna start being applied for
    things that are obviously true.
  *)
-
-Theorem inter_sym : forall s1 s2 : VarSet.t,
-    VarSet.inter s1 s2 = VarSet.inter s2 s1.
-Proof.
-  intros s1 s2. Admitted.
-
-Theorem union_sym : forall s1 s2 : VarSet.t,
-    VarSet.union s1 s2 = VarSet.union s2 s1.
-Proof.
-  intros s1 s2. Admitted.
-
-Theorem ctxu_sym : forall s1 s2 : ty_ctx,
-    ctxu s1 s2 = ctxu s2 s1.
-Proof. intros. Admitted.
-
-Theorem ctxu_assoc : forall s1 s2 s3 : ty_ctx,
-    ctxu s1 (ctxu s2 s3) = ctxu (ctxu s1 s2) s3.
-Proof. intros. Admitted.
-
-Theorem disj_vars_sym :
-  forall s1 s2 : ty_ctx,
-  forall disj_s1_s2 : (disj_vars s1 s2),
-    (disj_vars s2 s1).
-Proof. intros. unfold disj_vars in *. rewrite -> inter_sym. assumption.
-Qed.
 
 Theorem dvars_distrib :
   forall s1 s2 s3 : ty_ctx,
@@ -97,6 +70,13 @@ Theorem dvars_distrib :
     (and (disj_vars s1 s3) (disj_vars s2 s3)).
 Proof. intros. Admitted.
 
+Theorem ctxu_sym : forall s1 s2 : ty_ctx,
+    ctxu s1 s2 = ctxu s2 s1.
+Proof. intros. Admitted.
+
+Theorem ctxu_assoc : forall s1 s2 s3 : ty_ctx,
+    ctxu s1 (ctxu s2 s3) = ctxu (ctxu s1 s2) s3.
+Proof. intros. Admitted.
 
 Theorem ctxu_subset :
   forall g1 g2 g2a g2b : ty_ctx,
@@ -121,71 +101,3 @@ Theorem mutuallydisjoint_getsv2 :
   forall disj_g2_g2 : disj_vars g2 g3,
     disj_vars g1 (bound_variables (ctxu g2 g3)).
 Proof. Admitted.
-
-
-(* Theorem union_subset : forall s s1 s2 : VarSet.t, forall prf : s = VarSet.union s1 s2, *)
-(*     VarSet.Subset s1 s. *)
-(* Proof. intros s s1 s2 k. Admitted. *)
-
-(* Theorem subset_of_empty : forall s1 s2 : VarSet.t, forall s2_empty : VarSet.Empty s2, *)
-(*       forall s1_sub_s2 : VarSet.Subset s1 s2, *)
-(*         VarSet.Empty s1. *)
-(* Proof. intros. Admitted. *)
-
-(* Theorem inter_with_subset_is_subset_of_inter : forall s1 s2 s2a : VarSet.t, *)
-(*     forall s2a_sub_s2 : VarSet.Subset s2a s2, *)
-(*     VarSet.Subset (VarSet.inter s1 s2a) (VarSet.inter s1 s2). *)
-(* Proof. Admitted. *)
-
-(* Theorem disj_vars_over_sym1 : forall g1 g2 g3 : ty_ctx, *)
-(*     forall disj_12 : (disj_vars g1 g2), *)
-(*     disj_vars (bound_variables (ctxu g1 g2)) g3 = disj_vars g1 (bound_variables (ctxu g2 g3)). *)
-(* Proof. intros. Admitted. *)
-
-
-(* Set Nested Proofs Allowed. *)
-(* Set Printing Coercions. *)
-(* Lemma disj_vars_over_intersections : forall ga gb gc : ty_ctx, *)
-(*     forall disj_ga_gb : disj_vars ga gb, *)
-(*     forall disj_gab_c : disj_vars (bound_variables (ctxu ga gb)) gc, *)
-(*       disj_vars (bound_variables (ctxu ga gb)) gc = disj_vars (bound_variables (ctxu ga gc)) gb. *)
-(* Proof. intros. Admitted. *)
-
-(* Theorem disj_vars_sym : forall s1 s2 : VarSet.t, (iff (disj_vars s1 s2) (disj_vars s2 s1)). *)
-(* Proof. *)
-(*   intros s1 s2. unfold disj_vars. *)
-(*   unfold iff. *)
-(*   refine (conj _ _ ). *)
-(*   { intros h. rewrite <- inter_sym. assumption. } *)
-(*   { intros h. rewrite -> inter_sym. assumption. } *)
-(* Qed. *)
-
-(* Theorem disj_vars_subset : forall g gsub gsup : ty_ctx, *)
-(*     forall gsub_subset_gup : VarSet.Subset gsub gsup, *)
-(*       disj_vars g gsup -> disj_vars g gsub. *)
-(* Proof. *)
-(*   intros. unfold disj_vars in H. unfold disj_vars. *)
-(*   pose (ik := inter_with_subset_is_subset_of_inter (bound_variables g) *)
-(*        (bound_variables gsup) (bound_variables gsub) gsub_subset_gup). *)
-(*   exact (subset_of_empty (VarSet.inter (bound_variables g) (bound_variables gsub)) *)
-(*                          (VarSet.inter (bound_variables g) (bound_variables gsup)) *)
-(*                          H ik). *)
-(* Qed. *)
-
-(* Theorem ctx_union_sym : forall g1 g2 : ty_ctx, *)
-(*   (* This theorem is actually false, since contexts are currently backed with lists *) *)
-(*     forall p1 : (disj_vars g1 g2), forall p2 : (disj_vars g2 g1), *)
-(*     ctx_union g1 g2 p1 = ctx_union g2 g1 p2. *)
-(* Proof. *)
-(*   intros. *)
-(*   unfold ctx_union. *)
-(*   apply ctxu_sym. *)
-(* Qed. *)
-
-(* Theorem ctxu_unions_vars : forall g g1 g2 : ty_ctx, forall disj : disj_vars g1 g2, *)
-(*   forall gpartition : g = ctx_union g1 g2 disj, *)
-(*   (bound_variables g) = VarSet.union (bound_variables g1) (bound_variables g2). *)
-(* Proof. *)
-(*   intros g g1 g2 disj gpart. *)
-(*   unfold ctx_union in gpart. *)
-(* Admitted. *)
