lang.v
@@ -1,146 +1,62 @@
 Require Import lang_spec.
+Require Import lang_ops.
+Require Import lang_rels.
+Require Import typing_rels.
 Require Import EvalContexts.
 Require Import TypingContexts.
+Require Import VarSet.
 
 Require Import List.
 Import ListNotations.
 
-(* TODO There has to be a library function for this somewhere but I can't find it *)
-Fixpoint eq (n m : nat) : bool :=
-  match n, m with
-  | O, O => true
-  | S n', S m' => eq n' m'
-  | _, _ => false
-  end.
-
-Fixpoint substitute (e : expr) (s : expr) (x : var) : expr :=
-  match e with
-  | evar y =>
-    if eq x y then s else e
-  | (econst c) => e
-  | lam y T e' =>
-    if (eq x y) then e else lam y T (substitute e' s x)
-  | e1 @ e2 => (substitute e1 s x) @ (substitute e2 s x)
-  end.
-
-
-(* TODO I'm sure that I'm not defining free variables (in exprs and configs) correctly *)
-Fixpoint expr_freevars (e : expr) : VarSet.t :=
-  match e with
-  | evar y => VarSet.singleton y
-  | econst c => VarSet.empty
-  | lam y T e' => VarSet.diff (expr_freevars e') (VarSet.singleton y)
-  | e1 @ e2 => VarSet.union (expr_freevars e1) (expr_freevars e2)
-  end.
-
-Fixpoint config_freevars (c : config) : VarSet.t :=
-  match c with
-  | (c1 $$ c2) => VarSet.union (config_freevars c1) (config_freevars c2)
-  | x ** c => VarSet.diff (config_freevars c) (VarSet.singleton x)
-  | cellmake x v => VarSet.empty
-  | (x <- e) => VarSet.diff (expr_freevars e) (VarSet.singleton x)
-  | h ~ x => VarSet.empty
-  | h ~ used => VarSet.empty
-  end.
-
-Inductive expr_stepsto : expr -> expr -> Prop :=
-| step_beta x A e1 e2 : expr_stepsto ((lam x A e1) @ e2) (substitute e1 e2 x)
-| step_left e1 e2 e1' :
-    expr_stepsto e1 e1' -> expr_stepsto (e1 @ e2) (e1' @ e2)
-| step_right e1 e2 e2' :
-    expr_stepsto e2 e2' -> expr_stepsto (e1 @ e2) (e1 @ e2')
-| step_body x A e e' : expr_stepsto e e' -> expr_stepsto (lam x A e) (lam x A e')
-.
-
-(* Structural Congruence and Relations... *)
-
-Inductive structcong : config -> config -> Prop :=
-| cong_conc_commut (c1 c2 : config)
-  : structcong (c1 $$ c2) (c2 $$ c1)
-| cong_conc_assoc (c1 c2 c3 : config)
-  : structcong ((c1 $$ c2) $$ c3) (c1 $$ (c2 $$ c3))
-| cong_newplace_commut (c : config) (v1 v2 : var)
-  : structcong (v1 ** (v2 ** c)) (v2 ** (v1 ** c))
-| cong_newplace_distrib (c1 c2 : config) (v : var)
-                        (vfree : disj_vars v (config_freevars c2))
-  : structcong ((v ** c1) $$ c2) (v ** (c1 $$ c2))
-.
-
-(* TODO This needs to be condensed :| *)
-Inductive OperationalStepsTo : config -> config -> Prop :=
-| ost_beta (E : ctx_e) (lam_bind : var) (lam_bind_T : type) (lam_body : expr)
-           (v : val)
-  : OperationalStepsTo (SubInE ((lam lam_bind lam_bind_T lam_body) @ v) E)
-                       (SubInE (substitute lam_body v lam_bind) E)
-| ost_newthread (E : ctx_e) (v : val) (y : var)
-                (vfree : disj_vars y (config_freevars (SubInE v E)))
-  : OperationalStepsTo (SubInE (thread @ v) E)
-                       ((y ** (SubInE y E)) $$ (threadval y (v @ y)))
-| ost_future_deref (EF : ctx_ef) (y : var) (v : val)
-  : OperationalStepsTo ((SubInE y EF) $$ (threadval y v))
-                       ((SubInE v EF) $$ (threadval y v))
-| ost_handle_new (E : ctx_e) (v : val) (y z : var)
-                 (yfree : disj_vars y (config_freevars (SubInE v E)))
-                 (zfree : disj_vars z (config_freevars (SubInE v E)))
-  : OperationalStepsTo (SubInE (handle @ v) E)
-                       (y ** z ** (SubInE (v @ y @ z) E) $$ (z ~ y))
-| ost_handle_bind (E : ctx_e) (z y : var) (v : val)
-  : OperationalStepsTo ((SubInE (z @ v) E) $$ (z ~ y))
-                       ((SubInE unit E) $$ (threadval y v) $$ (usedhandle z))
-| ost_cell_new (E : ctx_e) (v : val) (y : var)
-               (yfree : disj_vars y (config_freevars (SubInE v E)))
-  : OperationalStepsTo (SubInE (cell @ v) E)
-                       (y ** ((SubInE y E) $$ y c= v))
-| ost_cell_exch (E : ctx_e) (y : var) (v1 v2 : val)
-  : OperationalStepsTo ((SubInE (exch @ y @ v1) E) $$ y c= v2)
-                       ((SubInE v2 E) $$ y c= v1)
-.
-
-Inductive expr_has_type : ty_ctx -> expr -> type -> Prop :=
-(* Constants *)
-(* TODO Folding typing of constants into typing of expressions might be suspect *)
-| ty_const_unit (g : ty_ctx) : expr_has_type g unit Unit
-| ty_const_thread (g : ty_ctx) (t : type) : expr_has_type g thread ((t >> t) >> t)
-| ty_const_handle (g : ty_ctx) (t1 t2 : type) : expr_has_type g handle ((t1 >> (t1 >> Unit) >> t2) >> t2)
-| ty_const_cell (g : ty_ctx) (t : type) : expr_has_type g cell (t >> (Ref t))
-| ty_const_exch (g : ty_ctx) (t : type) : expr_has_type g exch ((Ref t) >> t >> t)
-(* General Expressions *)
-| ty_var (g : ty_ctx) (x : var) (t : type) (xfree : disj_vars (VarSet.singleton x) g)
-  : expr_has_type (ctx_union (judge x t) g xfree) x t
-| ty_lam (g : ty_ctx) (x : var) (e : expr) (t1 t2 : type)
-         (xfree : disj_vars (VarSet.singleton x) g)
-         (_ : expr_has_type (ctx_union (judge x t1) g xfree) e t2)
-  : expr_has_type g (lam x t1 e) (t1 >> t2)
-| ty_app (g : ty_ctx) (e1 e2 : expr) (t1 t2 : type)
-         (_ : expr_has_type g e1 (t1 >> t2))
-         (_ : expr_has_type g e2 t2)
-  : expr_has_type g (e1 @ e2) t2
-.
-
-Inductive config_has_type : ty_ctx -> config -> ty_ctx -> Prop :=
-| ty_config_par (g g1 g2 : ty_ctx) (c1 c2 : config)
-                (g_g1 : disj_vars g g1) (g_g2 : disj_vars g g2) (g1_g2 : disj_vars g1 g2)
-                (p1 : config_has_type (ctx_union g g1 g_g1) c1 g2)
-                (p2 : config_has_type (ctx_union g g2 g_g2) c2 g1)
-  : config_has_type g (c1 $$ c2) (ctx_union g1 g2 g1_g2)
-| ty_config_ref (g : ty_ctx) (x : var) (t : type) (v : val)
-                (disj_prf : disj_vars (VarSet.singleton x) g)
-                (vprf : expr_has_type (ctx_union (judge x (Ref t)) g disj_prf) v t)
-  : config_has_type g (x c= v) (judge x (Ref t))
-| ty_config_reserveplace (g g': ty_ctx) (c : config) (x : var)
-                         (h : config_has_type g c g')
-  : config_has_type g (x ** c) (restrict_ty_ctx g' x)
-| ty_config_threadval (g : ty_ctx) (x : var) (t : type) (e : expr)
-                      (x_gfree : disj_vars (VarSet.singleton x) g)
-                      (h : expr_has_type (ctx_union (judge x t) g x_gfree) e t)
-  : config_has_type g (threadval x e) (judge x t)
-| ty_config_handledfut(g : ty_ctx) (x y : var) (t : type)
-                      (x_not_y : ~(x = y))
-  : config_has_type g (handledfut y x) [ (judge x t) ; (judge y (Arrow t Unit))]
-| ty_config_usedfut (g : ty_ctx) (y : var) (t : type)
-                    (y_gfree : disj_vars (VarSet.singleton y) g)
-  : config_has_type g (usedhandle y) [judge y (Arrow t Unit)]
-.
+Theorem config_gammas_disjoint
+  : forall G G' : ty_ctx,
+    forall C : config,
+    forall prf : config_has_type G C G',
+      disj_vars G G'.
+Proof.
+  intros G G' C prf.
+  induction prf.
+    + unfold ctx_union in *.
+      pose (prf := mutuallydisjoint_gets g1 g2 g g1_g2 (disj_vars_sym g g1 g_g1)).
+      apply disj_vars_sym in prf.
+      exact prf.
+      pose (prf3 := disj_vars_sym g g2 g_g2).
+      exact prf3.
+    + unfold disj_vars in *.
+      simpl in *.
+      rewrite -> (union_with_empty (VarSet.singleton x)).
+      rewrite -> axiom_inter_sym.
+      exact disj_prf.
+    + unfold disj_vars in *.
+      simpl.
+      pose (subset_prf := restriction_makes_subset g' x).
+      pose (bound_subset := inter_with_subset (bound_variables g)
+                                              (bound_variables g')
+                                              (bound_variables (g' -- x))
+                                              subset_prf).
+      exact (subset_of_empty (VarSet.inter (bound_variables g) (bound_variables g'))
+                             (VarSet.inter (bound_variables g) (bound_variables (g' -- x)))
+                             IHprf bound_subset).
+    + unfold coerce_judgement_to_ty_ctx in *.
+      simpl.
+      unfold disj_vars in *.
+      rewrite -> (union_with_empty (VarSet.singleton x)).
+      rewrite -> axiom_inter_sym.
+      exact x_gfree.
+    + simpl. rewrite -> union_with_empty.
+      pose (disj_xy := neq_means_disjoint x y x_not_y).
+      unfold disj_vars in *.
+      rewrite -> axiom_inter_sym in x_gfree.
+      rewrite -> axiom_inter_sym in y_gfree.
+      exact (mdisj_rassoc g (VarSet.singleton x) (VarSet.singleton y)
+                          x_gfree y_gfree disj_xy).
+    + unfold disj_vars in *.
+      simpl in *.
+      rewrite -> (union_with_empty (VarSet.singleton y)).
+      rewrite -> axiom_inter_sym.
+      exact y_gfree.
+Qed.
 
 Theorem Congruence_Preserves_Typing
   : forall g g': ty_ctx, forall c1 c2 : config,
@@ -220,10 +136,18 @@ Proof.
     pose (ty_prf_v1 := ty_config_reserveplace G g' c v1 ty_prf_all).
     pose (ty_prf_v1_v2 := ty_config_reserveplace G (g' -- v1) (v1 ** c) v2 ty_prf_v1).
 
-    rewrite -> axiom_restriction_commutative in ty_prf_v1_v2.
+    rewrite -> restriction_commutative in ty_prf_v1_v2.
     exact ty_prf_v1_v2.
 
-  + admit.
+  + inversion ty_prf as [g0 g1 g2subv c0 c3 disj_01 disj_02x disj_12x prf_g2subv prf_g1 | | | | | ].
+    clear H H0 H1 H2 c0 c3 ty_prf G' g0.
+    inversion prf_g2subv as [ | | g g2v c x prf_g2v | | | ].
+    (* unfold ctx_union in *. *)
+    (* rewrite <-H2 in *. *)
+    (* clear H H0 H1 H2 g x c g2subv. *)
+    clear H H0 H1 H2 g x c.
+    (* pose (goal := ty_config_reserveplace G (ctx_union g1 g2subv disj_12x) (c1 $$ c2) v). *)
+    (* pose (arg1 := ty_config_par G g1 g2subv c1 c2 disj_01 disj_02x disj_12x). *)
 Admitted.
 
 Theorem Subject_Reduction :
