VarSet.v
@@ -1,0 +1,58 @@
+From Coq Require Import MSets.
+Require Import lang_spec.
+
+Module VarSet := Make(Nat_as_OT).
+Definition disj_vars (s1 s2 : VarSet.t) := VarSet.Empty (VarSet.inter s1 s2).
+
+Fixpoint var_to_varset (v : var) : VarSet.t :=
+  VarSet.singleton v.
+Coercion var_to_varset : var >-> VarSet.t.
+
+Theorem axiom_inter_sym : forall s1 s2 : VarSet.t,
+    VarSet.inter s1 s2 = VarSet.inter s2 s1.
+Proof.
+  intros s1 s2. Admitted.
+
+Theorem axiom_union_sym : forall s1 s2 : VarSet.t,
+    VarSet.union s1 s2 = VarSet.union s2 s1.
+Proof.
+  intros s1 s2. Admitted.
+
+Theorem union_with_empty : forall s1 : VarSet.t,
+    VarSet.union s1 VarSet.empty = s1.
+Proof. Admitted.
+
+Theorem disj_vars_sym :
+  forall s1 s2 : VarSet.t,
+  forall disj_s1_s2 : (disj_vars s1 s2),
+    (disj_vars s2 s1).
+Proof. intros. unfold disj_vars in *. rewrite -> axiom_inter_sym. assumption.
+Qed.
+
+(* Elementary Set Theory Stuff? *)
+Theorem inter_with_subset :
+  forall s1 s2 sub_s2 : VarSet.t,
+  forall sub_prf : VarSet.Subset sub_s2 s2,
+    VarSet.Subset (VarSet.inter s1 sub_s2) (VarSet.inter s1 s2).
+Proof. Admitted.
+
+Theorem subset_of_empty :
+  forall s sub_s : VarSet.t,
+  forall s_empty : VarSet.Empty s,
+  forall sub_prf : VarSet.Subset sub_s s,
+    VarSet.Empty sub_s.
+Proof. Admitted.
+
+Theorem neq_means_disjoint :
+  forall x y : var,
+  forall neq_xy : ~(x = y),
+    VarSet.Empty (VarSet.inter (VarSet.singleton x) (VarSet.singleton y)).
+Proof. Admitted.
+
+Theorem mdisj_rassoc :
+  forall s1 s2 s3 : VarSet.t,
+  forall disj_s12 : VarSet.Empty (VarSet.inter s1 s2),
+  forall disj_s13 : VarSet.Empty (VarSet.inter s1 s3),
+  forall disj_s23 : VarSet.Empty (VarSet.inter s2 s3),
+    VarSet.Empty (VarSet.inter s1 (VarSet.union s2 s3)).
+Proof. Admitted.
