lang_ops.v
@@ -1,0 +1,40 @@
+Require Import lang_spec.
+Require Import VarSet.
+
+(* TODO There has to be a library function for this somewhere but I can't find it *)
+Fixpoint eq (n m : nat) : bool :=
+  match n, m with
+  | O, O => true
+  | S n', S m' => eq n' m'
+  | _, _ => false
+  end.
+
+Fixpoint substitute (e : expr) (s : expr) (x : var) : expr :=
+  match e with
+  | evar y =>
+    if eq x y then s else e
+  | (econst c) => e
+  | lam y T e' =>
+    if (eq x y) then e else lam y T (substitute e' s x)
+  | e1 @ e2 => (substitute e1 s x) @ (substitute e2 s x)
+  end.
+
+
+(* TODO I'm sure that I'm not defining free variables (in exprs and configs) correctly *)
+Fixpoint expr_freevars (e : expr) : VarSet.t :=
+  match e with
+  | evar y => VarSet.singleton y
+  | econst c => VarSet.empty
+  | lam y T e' => VarSet.diff (expr_freevars e') (VarSet.singleton y)
+  | e1 @ e2 => VarSet.union (expr_freevars e1) (expr_freevars e2)
+  end.
+
+Fixpoint config_freevars (c : config) : VarSet.t :=
+  match c with
+  | (c1 $$ c2) => VarSet.union (config_freevars c1) (config_freevars c2)
+  | x ** c => VarSet.diff (config_freevars c) (VarSet.singleton x)
+  | cellmake x v => VarSet.empty
+  | (x <- e) => VarSet.diff (expr_freevars e) (VarSet.singleton x)
+  | h ~ x => VarSet.empty
+  | h ~ used => VarSet.empty
+  end.
